nsl.v
@@ -30,21 +30,16 @@ Definition nsl_init : expr :=
 Definition nsl_resp : expr :=
   pk_auth_resp N nsl_gen_keys nsl_mk_sess_key.
 
-Class NSL := {
-  session : role → term → term → term → iProp;
-}.
-
-Context `{!NSL}.
-
 Definition nsl_ctx : iProp :=
   session.session_ctx (@nonce_meta _ _) N
-    (λ rl nI nR '(kI, kR), session rl kI kR nI).
+    (λ rl nI nR (_ : term * term), True)%I.
 
 Definition nsl_resp_accepted kI kR sI sR : iProp :=
   session.session (@nonce_meta _ heap) N Resp sI sR (kI, kR).
 
 Definition nsl_init_finished sR : iProp := □ ∀ kI kR sI,
   session.session (@nonce_meta _ _) N Resp sI sR (kI, kR) →
+  secret_of sI kI kR ∧
   session.session (@nonce_meta _ _) N Init sI sR (kI, kR).
 
 Program Instance PK_NSL : PK N := {
@@ -57,12 +52,14 @@ Program Instance PK_NSL : PK N := {
   resp_accepted := nsl_resp_accepted;
 
   resp_waiting kI kR sI nR sR := (
-    ⌜sR = nR⌝ ∧ nonce_meta_token nR (↑N)
+    ⌜sR = nR⌝ ∧
+    waiting_for_peer (@nonce_meta _ heap)
+                     N (λ _ _ _ _, True)%I Resp sI nR (kI, kR)
   )%I;
 
   init_finished := nsl_init_finished;
 
-  session rl kI kR kS := session rl kI kR kS;
+  session rl kI kR kS := True%I;
 
   init_gen_keys := nsl_gen_keys;
   init_mk_sess_key := nsl_mk_sess_key;
@@ -83,12 +80,47 @@ by rewrite /secret_of bi.intuitionistic_intuitionistically.
 Qed.
 
 Next Obligation.
-iIntros "%E %kI %kR %nI %sI %sR % #? #accepted %Ψ !> [-> token] post".
+iIntros "%E %kI %kR %nI %sI %sR % #ctx #s_nI _ #p_nI #s_sR #p_sR".
+iIntros "[#fail|#sessR] %Ψ !> (-> & token) post".
+  rewrite /nsl_mk_sess_key. wp_pures. iModIntro. iApply "post".
+  by do !iSplit; eauto.
+iMod (session_begin _ Init _ sR (kI, kR) with "ctx [//] token")
+  as "[#sessI end]" => //.
+(* This condition should be more interesting eventually *)
+iMod ("end" with "[//] sessR") as "end".
+rewrite /nsl_mk_sess_key. wp_pures. iModIntro. iApply "post".
+do !iSplit; eauto. iRight.
+iIntros "!> %kI' %kR' %nI' #sessR'".
+iPoseProof (session_agree with "sessR' sessR") as "%e" => //.
+case: e => -> -> ->. by eauto.
+Qed.
 
+Next Obligation.
+iIntros "%E %kI %kR %nI % #ctx #s_nI _ !> %Ψ _ post".
+rewrite /nsl_gen_keys. wp_pures. wp_bind (mknonce _).
+iApply (wp_mknonce _ (λ _, corruption kI kR) (λ _, True)%I).
+iIntros "%nR #s_nR #p_nR _ token".
+rewrite bi.intuitionistic_intuitionistically.
+rewrite (term_meta_token_difference _ (↑N)) //.
+iDestruct "token" as "[token _]". wp_pures.
+iApply "post".
+iMod (session_begin _ Resp nI nR (kI, kR) with "ctx [//] token")
+  as "[#sessR waiting]" => //.
+by iModIntro; do 5!iSplit => //.
+Qed.
 
+Next Obligation.
+iIntros "%E %kI %kR %sI %nR %sR % #ctx #s_sI #p_sI #s_nR #s_sR #p_sR".
+iIntros "#accepted #finishedI !> %Ψ [-> waiting] post".
+rewrite /nsl_mk_sess_key. wp_pures.
+iDestruct "finishedI" as "[fail|#finishedI]".
+  iModIntro. iApply "post". do!iSplit; eauto.
+  iModIntro. iSplit; eauto.
+  iIntros "_". by iApply "p_sI".
+iPoseProof ("finishedI" with "accepted") as "{p_sI} [p_sI finished]".
+(* This step should be more interesting eventually *)
+iMod ("waiting" with "[//] finished") as "finishedR".
+iModIntro. iApply "post". by eauto.
+Qed.
 
 End NSL.
-
-Arguments nsl_ctx {Σ _ _} term_meta {_} N P γ.
-Arguments wp_nsl_init {Σ _ _ _ _ _ _ N} P Q.
-Arguments wp_nsl_resp {Σ _ _ _ _ _ _ N} P Q.
